format-version: 1.2
data-version: ohpi/releases/2019-04-12/imports/ino_import.owl
ontology: ohpi/imports/ino_import
owl-axioms: Prefix(owl:=<http://www.w3.org/2002/07/owl#>)\nPrefix(rdf:=<http://www.w3.org/1999/02/22-rdf-syntax-ns#>)\nPrefix(xml:=<http://www.w3.org/XML/1998/namespace>)\nPrefix(xsd:=<http://www.w3.org/2001/XMLSchema#>)\nPrefix(rdfs:=<http://www.w3.org/2000/01/rdf-schema#>)\n\n\nOntology(\nDeclaration(Class(<http://purl.obolibrary.org/obo/BFO_0000001>))\nDeclaration(Class(<http://purl.obolibrary.org/obo/INO_0000002>))\nDeclaration(Class(<http://purl.obolibrary.org/obo/INO_0000015>))\nDeclaration(ObjectProperty(<http://purl.obolibrary.org/obo/RO_0000057>))\nDeclaration(ObjectProperty(<http://purl.obolibrary.org/obo/RO_0000087>))\nDeclaration(AnnotationProperty(<http://purl.obolibrary.org/obo/BFO_0000179>))\nDeclaration(AnnotationProperty(<http://purl.obolibrary.org/obo/BFO_0000180>))\n############################\n#   Annotation Properties\n############################\n\n# Annotation Property: <http://purl.obolibrary.org/obo/BFO_0000179> (BFO OWL specification label)\n\nSubAnnotationPropertyOf(<http://purl.obolibrary.org/obo/BFO_0000179> rdfs:label)\n\n# Annotation Property: <http://purl.obolibrary.org/obo/BFO_0000180> (BFO CLIF specification label)\n\nSubAnnotationPropertyOf(<http://purl.obolibrary.org/obo/BFO_0000180> rdfs:label)\n\n\n\n############################\n#   Classes\n############################\n\n# Class: <http://purl.obolibrary.org/obo/INO_0000002> (interaction)\n\nSubClassOf(<http://purl.obolibrary.org/obo/INO_0000002> ObjectSomeValuesFrom(<http://purl.obolibrary.org/obo/RO_0000057> ObjectIntersectionOf(<http://purl.obolibrary.org/obo/BFO_0000001> ObjectSomeValuesFrom(<http://purl.obolibrary.org/obo/RO_0000087> <http://purl.obolibrary.org/obo/INO_0000015>))))\n\n\n)

[Term]
id: BFO:0000001
name: entity
property_value: BFO:0000179 "entity" xsd:string
property_value: BFO:0000180 "Entity" xsd:string
property_value: IAO:0000112 "Julius Caesar" xsd:string
property_value: IAO:0000112 "the Second World War" xsd:string
property_value: IAO:0000112 "Verdi’s Requiem" xsd:string
property_value: IAO:0000112 "your body mass index" xsd:string
property_value: IAO:0000116 "BFO 2 Reference: In all areas of empirical inquiry we encounter general terms of two sorts. First are general terms which refer to universals or types:animaltuberculosissurgical procedurediseaseSecond, are general terms used to refer to groups of entities which instantiate a given universal but do not correspond to the extension of any subuniversal of that universal because there is nothing intrinsic to the entities in question by virtue of which they – and only they – are counted as belonging to the given group. Examples are: animal purchased by the Emperortuberculosis diagnosed on a Wednesdaysurgical procedure performed on a patient from Stockholmperson identified as candidate for clinical trial #2056-555person who is signatory of Form 656-PPVpainting by Leonardo da VinciSuch terms, which represent what are called ‘specializations’ in [81" xsd:string
property_value: IAO:0000116 "Entity doesn't have a closure axiom because the subclasses don't necessarily exhaust all possibilites. For example Werner Ceusters 'portions of reality' include 4 sorts, entities (as BFO construes them), universals, configurations, and relations. It is an open question as to whether entities as construed in BFO will at some point also include these other portions of reality. See, for example, 'How to track absolutely everything' at http://www.referent-tracking.com/_RTU/papers/CeustersICbookRevised.pdf" xsd:string
property_value: IAO:0000412 http://purl.obolibrary.org/obo/bfo.owl
property_value: IAO:0000412 http://purl.obolibrary.org/obo/ino.owl
property_value: IAO:0000600 "An entity is anything that exists or has existed or will exist. (axiom label in BFO2 Reference: [001-001])" xsd:string
property_value: isDefinedBy http://purl.obolibrary.org/obo/bfo.owl

[Term]
id: BFO:0000002
name: continuant
def: "An entity that exists in full at any time in which it exists at all, persists through time while maintaining its identity and has no temporal parts." []
is_a: BFO:0000001 ! entity
property_value: BFO:0000179 "continuant" xsd:string
property_value: BFO:0000180 "Continuant" xsd:string
property_value: IAO:0000116 "BFO 2 Reference: Continuant entities are entities which can be sliced to yield parts only along the spatial dimension, yielding for example the parts of your table which we call its legs, its top, its nails. ‘My desk stretches from the window to the door. It has spatial parts, and can be sliced (in space) in two. With respect to time, however, a thing is a continuant.’ [60, p. 240" xsd:string
property_value: IAO:0000116 "Continuant doesn't have a closure axiom because the subclasses don't necessarily exhaust all possibilites. For example, in an expansion involving bringing in some of Ceuster's other portions of reality, questions are raised as to whether universals are continuants" xsd:string
property_value: IAO:0000412 http://purl.obolibrary.org/obo/bfo.owl
property_value: IAO:0000412 http://purl.obolibrary.org/obo/ino.owl
property_value: IAO:0000412 http://purl.obolibrary.org/obo/ro.owl
property_value: IAO:0000600 "A continuant is an entity that persists, endures, or continues to exist through time while maintaining its identity. (axiom label in BFO2 Reference: [008-002])" xsd:string
property_value: IAO:0000601 "if b is a continuant and if, for some t, c has_continuant_part b at t, then c is a continuant. (axiom label in BFO2 Reference: [126-001])" xsd:string
property_value: IAO:0000601 "if b is a continuant and if, for some t, cis continuant_part of b at t, then c is a continuant. (axiom label in BFO2 Reference: [009-002])" xsd:string
property_value: IAO:0000601 "if b is a material entity, then there is some temporal interval (referred to below as a one-dimensional temporal region) during which b exists. (axiom label in BFO2 Reference: [011-002])" xsd:string
property_value: IAO:0000602 "(forall (x y) (if (and (Continuant x) (exists (t) (continuantPartOfAt y x t))) (Continuant y))) // axiom label in BFO2 CLIF: [009-002] " xsd:string
property_value: IAO:0000602 "(forall (x y) (if (and (Continuant x) (exists (t) (hasContinuantPartOfAt y x t))) (Continuant y))) // axiom label in BFO2 CLIF: [126-001] " xsd:string
property_value: IAO:0000602 "(forall (x) (if (Continuant x) (Entity x))) // axiom label in BFO2 CLIF: [008-002] " xsd:string
property_value: IAO:0000602 "(forall (x) (if (Material Entity x) (exists (t) (and (TemporalRegion t) (existsAt x t))))) // axiom label in BFO2 CLIF: [011-002] " xsd:string
property_value: isDefinedBy http://purl.obolibrary.org/obo/bfo.owl

[Term]
id: BFO:0000015
name: process
def: "An occurrent that has temporal proper parts and for some time t, p s-depends_on some material entity at t." []
def: "p is a process = Def. p is an occurrent that has temporal proper parts and for some time t, p s-depends_on some material entity at t. (axiom label in BFO2 Reference: [083-003])" []
property_value: BFO:0000179 "process" xsd:string
property_value: BFO:0000180 "Process" xsd:string
property_value: IAO:0000112 "a process of cell-division, \\ a beating of the heart" xsd:string
property_value: IAO:0000112 "a process of meiosis" xsd:string
property_value: IAO:0000112 "a process of sleeping" xsd:string
property_value: IAO:0000112 "the course of a disease" xsd:string
property_value: IAO:0000112 "the flight of a bird" xsd:string
property_value: IAO:0000112 "the life of an organism" xsd:string
property_value: IAO:0000112 "your process of aging." xsd:string
property_value: IAO:0000116 "BFO 2 Reference: The realm of occurrents is less pervasively marked by the presence of natural units than is the case in the realm of independent continuants. Thus there is here no counterpart of ‘object’. In BFO 1.0 ‘process’ served as such a counterpart. In BFO 2.0 ‘process’ is, rather, the occurrent counterpart of ‘material entity’. Those natural – as contrasted with engineered, which here means: deliberately executed – units which do exist in the realm of occurrents are typically either parasitic on the existence of natural units on the continuant side, or they are fiat in nature. Thus we can count lives; we can count football games; we can count chemical reactions performed in experiments or in chemical manufacturing. We cannot count the processes taking place, for instance, in an episode of insect mating behavior.Even where natural units are identifiable, for example cycles in a cyclical process such as the beating of a heart or an organism’s sleep/wake cycle, the processes in question form a sequence with no discontinuities (temporal gaps) of the sort that we find for instance where billiard balls or zebrafish or planets are separated by clear spatial gaps. Lives of organisms are process units, but they too unfold in a continuous series from other, prior processes such as fertilization, and they unfold in turn in continuous series of post-life processes such as post-mortem decay. Clear examples of boundaries of processes are almost always of the fiat sort (midnight, a time of death as declared in an operating theater or on a death certificate, the initiation of a state of war)" xsd:string
property_value: IAO:0000412 http://purl.obolibrary.org/obo/bfo.owl
property_value: IAO:0000412 http://purl.obolibrary.org/obo/ino.owl
property_value: IAO:0000412 http://purl.obolibrary.org/obo/ro.owl
property_value: IAO:0000602 "(iff (Process a) (and (Occurrent a) (exists (b) (properTemporalPartOf b a)) (exists (c t) (and (MaterialEntity c) (specificallyDependsOnAt a c t))))) // axiom label in BFO2 CLIF: [083-003] " xsd:string
property_value: isDefinedBy http://purl.obolibrary.org/obo/bfo.owl

[Term]
id: BFO:0000017
name: realizable entity
def: "A specifically dependent continuant  that inheres in continuant  entities and are not exhibited in full at every time in which it inheres in an entity or group of entities. The exhibition or actualization of a realizable entity is a particular manifestation, functioning or process that occurs under certain circumstances." []
is_a: BFO:0000020 ! specifically dependent continuant
property_value: BFO:0000179 "realizable" xsd:string
property_value: BFO:0000180 "RealizableEntity" xsd:string
property_value: IAO:0000112 "the disposition of this piece of metal to conduct electricity." xsd:string
property_value: IAO:0000112 "the disposition of your blood to coagulate" xsd:string
property_value: IAO:0000112 "the function of your reproductive organs" xsd:string
property_value: IAO:0000112 "the role of being a doctor" xsd:string
property_value: IAO:0000112 "the role of this boundary to delineate where Utah and Colorado meet" xsd:string
property_value: IAO:0000412 http://purl.obolibrary.org/obo/bfo.owl
property_value: IAO:0000412 http://purl.obolibrary.org/obo/ino.owl
property_value: IAO:0000412 http://purl.obolibrary.org/obo/ro.owl
property_value: IAO:0000600 "To say that b is a realizable entity is to say that b is a specifically dependent continuant that inheres in some independent continuant which is not a spatial region and is of a type instances of which are realized in processes of a correlated type. (axiom label in BFO2 Reference: [058-002])" xsd:string
property_value: IAO:0000601 "All realizable dependent continuants have independent continuants that are not spatial regions as their bearers. (axiom label in BFO2 Reference: [060-002])" xsd:string
property_value: IAO:0000602 "(forall (x t) (if (RealizableEntity x) (exists (y) (and (IndependentContinuant y) (not (SpatialRegion y)) (bearerOfAt y x t))))) // axiom label in BFO2 CLIF: [060-002] " xsd:string
property_value: IAO:0000602 "(forall (x) (if (RealizableEntity x) (and (SpecificallyDependentContinuant x) (exists (y) (and (IndependentContinuant y) (not (SpatialRegion y)) (inheresIn x y)))))) // axiom label in BFO2 CLIF: [058-002] " xsd:string
property_value: isDefinedBy http://purl.obolibrary.org/obo/bfo.owl

[Term]
id: BFO:0000020
name: specifically dependent continuant
def: "A continuant that inheres in or is borne by other entities. Every instance of A requires some specific instance of B which must always be the same." []
def: "b is a specifically dependent continuant = Def. b is a continuant & there is some independent continuant c which is not a spatial region and which is such that b s-depends_on c at every time t during the course of b’s existence. (axiom label in BFO2 Reference: [050-003])" []
is_a: BFO:0000002 ! continuant
property_value: BFO:0000179 "sdc" xsd:string
property_value: BFO:0000180 "SpecificallyDependentContinuant" xsd:string
property_value: IAO:0000112 "of one-sided specifically dependent continuants: the mass of this tomato" xsd:string
property_value: IAO:0000112 "of relational dependent continuants (multiple bearers): John’s love for Mary, the ownership relation between John and this statue, the relation of authority between John and his subordinates." xsd:string
property_value: IAO:0000112 "Reciprocal specifically dependent continuants: the function of this key to open this lock and the mutually dependent disposition of this lock: to be opened by this key" xsd:string
property_value: IAO:0000112 "the disposition of this fish to decay" xsd:string
property_value: IAO:0000112 "the function of this heart: to pump blood" xsd:string
property_value: IAO:0000112 "the mutual dependence of proton donors and acceptors in chemical reactions [79" xsd:string
property_value: IAO:0000112 "the mutual dependence of the role predator and the role prey as played by two organisms in a given interaction" xsd:string
property_value: IAO:0000112 "the pink color of a medium rare piece of grilled filet mignon at its center" xsd:string
property_value: IAO:0000112 "the role of being a doctor" xsd:string
property_value: IAO:0000112 "the shape of this hole." xsd:string
property_value: IAO:0000112 "the smell of this portion of mozzarella" xsd:string
property_value: IAO:0000116 "Specifically dependent continuant doesn't have a closure axiom because the subclasses don't necessarily exhaust all possibilites. We're not sure what else will develop here, but for example there are questions such as what are promises, obligation, etc." xsd:string
property_value: IAO:0000412 http://purl.obolibrary.org/obo/bfo.owl
property_value: IAO:0000412 http://purl.obolibrary.org/obo/ino.owl
property_value: IAO:0000412 http://purl.obolibrary.org/obo/ro.owl
property_value: IAO:0000602 "(iff (SpecificallyDependentContinuant a) (and (Continuant a) (forall (t) (if (existsAt a t) (exists (b) (and (IndependentContinuant b) (not (SpatialRegion b)) (specificallyDependsOnAt a b t))))))) // axiom label in BFO2 CLIF: [050-003] " xsd:string
property_value: isDefinedBy http://purl.obolibrary.org/obo/bfo.owl

[Term]
id: BFO:0000023
name: role
def: "A realizable entity  the manifestation of which brings about some result or end that is not essential to a continuant  in virtue of the kind of thing that it is but that can be served or participated in by that kind of continuant  in some kinds of natural, social or institutional contexts." []
is_a: BFO:0000017 ! realizable entity
property_value: BFO:0000179 "role" xsd:string
property_value: BFO:0000180 "Role" xsd:string
property_value: IAO:0000112 "John’s role of husband to Mary is dependent on Mary’s role of wife to John, and both are dependent on the object aggregate comprising John and Mary as member parts joined together through the relational quality of being married." xsd:string
property_value: IAO:0000112 "the priest role" xsd:string
property_value: IAO:0000112 "the role of a boundary to demarcate two neighboring administrative territories" xsd:string
property_value: IAO:0000112 "the role of a building in serving as a military target" xsd:string
property_value: IAO:0000112 "the role of a stone in marking a property boundary" xsd:string
property_value: IAO:0000112 "the role of subject in a clinical trial" xsd:string
property_value: IAO:0000112 "the student role" xsd:string
property_value: IAO:0000116 "BFO 2 Reference: One major family of examples of non-rigid universals involves roles, and ontologies developed for corresponding administrative purposes may consist entirely of representatives of entities of this sort. Thus ‘professor’, defined as follows,b instance_of professor at t =Def. there is some c, c instance_of professor role & c inheres_in b at t.denotes a non-rigid universal and so also do ‘nurse’, ‘student’, ‘colonel’, ‘taxpayer’, and so forth. (These terms are all, in the jargon of philosophy, phase sortals.) By using role terms in definitions, we can create a BFO conformant treatment of such entities drawing on the fact that, while an instance of professor may be simultaneously an instance of trade union member, no instance of the type professor role is also (at any time) an instance of the type trade union member role (any more than any instance of the type color is at any time an instance of the type length).If an ontology of employment positions should be defined in terms of roles following the above pattern, this enables the ontology to do justice to the fact that individuals instantiate the corresponding universals –  professor, sergeant, nurse – only during certain phases in their lives." xsd:string
property_value: IAO:0000412 http://purl.obolibrary.org/obo/bfo.owl
property_value: IAO:0000412 http://purl.obolibrary.org/obo/ido.owl
property_value: IAO:0000412 http://purl.obolibrary.org/obo/ino.owl
property_value: IAO:0000412 http://purl.obolibrary.org/obo/ro.owl
property_value: IAO:0000600 "b is a role means: b is a realizable entity & b exists because there is some single bearer that is in some special physical, social, or institutional set of circumstances in which this bearer does not have to be& b is not such that, if it ceases to exist, then the physical make-up of the bearer is thereby changed. (axiom label in BFO2 Reference: [061-001])" xsd:string
property_value: IAO:0000602 "(forall (x) (if (Role x) (RealizableEntity x))) // axiom label in BFO2 CLIF: [061-001] " xsd:string
property_value: isDefinedBy http://purl.obolibrary.org/obo/bfo.owl

[Term]
id: INO:0000002
name: interaction
def: "Interaction is a processual entity that has two or more participants (i.e., interactors) that have an effect upon one another. " []
is_a: BFO:0000015 ! process
property_value: IAO:0000117 "YH, ZX" xsd:string
property_value: IAO:0000412 http://purl.obolibrary.org/obo/ino.owl
property_value: INO:0000006 "interact, interacted, interacting, interaction, interaction, interactor, interactors, interacts, participates; plays a role, contribute, contributed, contributes, contributing, engagement, engagements, engages, engaging, involve, involved, involves, involving, act, acted, acting, acts" xsd:string

[Term]
id: INO:0000005
name: regulator role
def: "an regulator role that is borne by a material entity that regulates an interaction." []
is_a: INO:0000015 ! interactor role
property_value: IAO:0000117 "YH" xsd:string
property_value: IAO:0000412 http://purl.obolibrary.org/obo/ino.owl

[Term]
id: INO:0000009
name: input interactor role
def: "an interactor role that is borne by a material entity that acts as an input of an interaction." []
is_a: INO:0000015 ! interactor role
property_value: IAO:0000117 "YH, ZX" xsd:string
property_value: IAO:0000118 "interaction input role" xsd:string
property_value: IAO:0000412 http://purl.obolibrary.org/obo/ino.owl

[Term]
id: INO:0000010
name: output interactor role
def: "an interactor role that is borne by a material entity that acts as an output of an interaction." []
is_a: INO:0000015 ! interactor role
property_value: IAO:0000117 "YH, ZX" xsd:string
property_value: IAO:0000118 "interaction output role" xsd:string
property_value: IAO:0000412 http://purl.obolibrary.org/obo/ino.owl

[Term]
id: INO:0000011
name: activator role
def: "a positive regulator role that is borne by a material entity that activates an interaction." []
is_a: INO:0000134 ! positive regulator role
property_value: IAO:0000117 "YH" xsd:string
property_value: IAO:0000412 http://purl.obolibrary.org/obo/ino.owl

[Term]
id: INO:0000015
name: interactor role
def: "a role that is borne by a material entity to act as a participant in an interaction process." []
is_a: BFO:0000023 ! role
relationship: BFO:0000054 INO:0000002 ! realized in interaction
property_value: IAO:0000117 "YH, ZX" xsd:string
property_value: IAO:0000412 http://purl.obolibrary.org/obo/ino.owl

[Term]
id: INO:0000069
name: chemical reaction catalyst role
def: "an interactor role that is played by a material entity that starts or speeds up a chemical reaction while undergoing no permanent change itself." []
is_a: INO:0000015 ! interactor role
property_value: IAO:0000117 "YH" xsd:string
property_value: IAO:0000412 http://purl.obolibrary.org/obo/ino.owl

[Term]
id: INO:0000134
name: positive regulator role
def: "an interactor role that is borne by a material entity that positively regulates an interaction." []
is_a: INO:0000005 ! regulator role
property_value: IAO:0000117 "YH" xsd:string
property_value: IAO:0000412 http://purl.obolibrary.org/obo/ino.owl

[Term]
id: INO:0000137
name: negative regulator role
def: "an interactor role that is borne by a material entity that negatively regulates an interaction." []
is_a: INO:0000005 ! regulator role
property_value: IAO:0000117 "YH" xsd:string
property_value: IAO:0000412 http://purl.obolibrary.org/obo/ino.owl

[Term]
id: INO:0000145
name: deactivator role
def: "a negative regulator role that is borne by a material entity that deactivates,  inhibits, blocks, or disrupts the action of a biological agent (e.g., enzyme)." []
is_a: INO:0000137 ! negative regulator role
property_value: IAO:0000117 "YH" xsd:string
property_value: IAO:0000412 http://purl.obolibrary.org/obo/ino.owl

[Term]
id: INO:0000147
name: motivator role
def: "an input interactor role that is borne by a material entity that motivates a process." []
is_a: INO:0000009 ! input interactor role
property_value: IAO:0000117 "Oliver He" xsd:string
property_value: IAO:0000119 https://en.wikipedia.org/wiki/Motivation#Herzberg's_two-factor_theory xsd:string
property_value: IAO:0000412 http://purl.obolibrary.org/obo/ino.owl

[Term]
id: INO:0000150
name: hygiene factor role
def: "an input interactor role that is borne by a material entity (e.g. status, job security, salary and fringe benefits) that do not motivate if present, but, if absent, result in demotivation." []
is_a: INO:0000009 ! input interactor role
property_value: IAO:0000117 "Oliver He" xsd:string
property_value: IAO:0000119 https://en.wikipedia.org/wiki/Motivation#Herzberg's_two-factor_theory xsd:string
property_value: IAO:0000412 http://purl.obolibrary.org/obo/ino.owl

[Typedef]
id: BFO:0000054
name: realized in

[Typedef]
id: RO:0000057
name: has participant

[Typedef]
id: RO:0000087
name: has role

